Two more Basic examples

platform/Depl/examples/Basic.v
@@ -18,7 +18,7 @@ Definition unused := dmodule "m" {{
 
 Theorem unusedOk : moduleOk unused.
 Proof.
-  depl; auto.
+  depl.
 Qed.
 
 
@@ -39,5 +39,53 @@ Definition unit := dmodule "m" {{
 
 Theorem unitOk : moduleOk unit.
 Proof.
-  depl; auto.
+  depl.
+Qed.
+
+
+(** * Lists with a degenerate specification *)
+
+Definition list := dmodule "m" {{
+  dtype "list" = {{ #"nil"("dummy";) "this" = |^_, !tt|
+                    with #"cons"("hd";"tl") "this" = |^_, !tt| }}
+  with dfunction "f" [
+    ARGS()
+    PRE Emp
+    POST #"list"(|^_, !tt|, "result")
+  ]
+    Locals "ret" in
+    "ret" <-- #"nil"(0);;
+    "ret" <-- #"cons"(42, "ret");;
+    "ret" <-- #"cons"(23, "ret");;
+    Return "ret"
+  end
+}}.
+
+Theorem listOk : moduleOk list.
+Proof.
+  depl.
+Qed.
+
+
+(** * Binary trees with a degenerate specification *)
+
+Definition tree := dmodule "m" {{
+  dtype "tree" = {{ #"leaf"("dummy";) "this" = |^_, !tt|
+                    with #"node"("data";"left","right") "this" = |^_, !tt| }}
+  with dfunction "f" [
+    ARGS()
+    PRE Emp
+    POST #"tree"(|^_, !tt|, "result")
+  ]
+    Locals "left", "right", "ret" in
+    "left" <-- #"leaf"(0);;
+    "right" <-- #"leaf"(0);;
+    "ret" <-- #"node"(42, "left", "right");;
+    Return "ret"
+  end
+}}.
+
+Theorem treeOk : moduleOk tree.
+Proof.
+  depl.
 Qed.
